WebAssembly/Wasm.thy
@@ -101,7 +101,7 @@ and       s_typing :: "[s, (t list) option, f, e list, t list] \<Rightarrow> boo
   (* trap *)
 | "\<S>\<bullet>\<C> \<turnstile> [Trap] : tf"
   (* local *)
-| "\<lbrakk>\<S>\<bullet>Some ts \<tturnstile> f;es : ts; length ts = n\<rbrakk> \<Longrightarrow> \<S>\<bullet>\<C> \<turnstile> [Local n f es] : ([] _> ts)"
+| "\<lbrakk>\<S>\<bullet>Some ts \<tturnstile> f;es : ts; length ts = n\<rbrakk> \<Longrightarrow> \<S>\<bullet>\<C> \<turnstile> [Frame n f es] : ([] _> ts)"
   (* invoke *)
 | "\<lbrakk>cl_typing \<S> cl tf\<rbrakk> \<Longrightarrow> \<S>\<bullet>\<C>  \<turnstile> [Invoke cl] : tf"
   (* label *)
@@ -167,10 +167,10 @@ inductive reduce_simple :: "[e list, e list] \<Rightarrow> bool" ("\<lparr>_\<rp
 | br_table:"\<lbrakk>length is > (nat_of_int c)\<rbrakk> \<Longrightarrow> \<lparr>[$C (ConstInt32 c), $(Br_table is i)]\<rparr> \<leadsto> \<lparr>[$(Br (is!(nat_of_int c)))]\<rparr>"
 | br_table_length:"\<lbrakk>length is \<le> (nat_of_int c)\<rbrakk> \<Longrightarrow> \<lparr>[$C (ConstInt32 c), $(Br_table is i)]\<rparr> \<leadsto> \<lparr>[$(Br i)]\<rparr>"
   \<comment> \<open>\<open>local\<close>\<close>
-| local_const:"\<lparr>[Local n f ($C* vs)]\<rparr> \<leadsto> \<lparr>($C* vs)\<rparr>"
-| local_trap:"\<lparr>[Local n f [Trap]]\<rparr> \<leadsto> \<lparr>[Trap]\<rparr>"
+| local_const:"\<lparr>[Frame n f ($C* vs)]\<rparr> \<leadsto> \<lparr>($C* vs)\<rparr>"
+| local_trap:"\<lparr>[Frame n f [Trap]]\<rparr> \<leadsto> \<lparr>[Trap]\<rparr>"
   \<comment> \<open>\<open>return\<close>\<close>
-| return:"\<lbrakk>length vs = n; Lfilled j lholed (($C* vs) @ [$Return]) es\<rbrakk>  \<Longrightarrow> \<lparr>[Local n f es]\<rparr> \<leadsto> \<lparr>($C* vs)\<rparr>"
+| return:"\<lbrakk>length vs = n; Lfilled j lholed (($C* vs) @ [$Return]) es\<rbrakk>  \<Longrightarrow> \<lparr>[Frame n f es]\<rparr> \<leadsto> \<lparr>($C* vs)\<rparr>"
   \<comment> \<open>\<open>tee_local\<close>\<close>
 | tee_local:"\<lparr>[$C v, $(Tee_local i)]\<rparr> \<leadsto> \<lparr>[$C v, $C v, $(Set_local i)]\<rparr>"
 | trap:"\<lbrakk>es \<noteq> [Trap]; Lfilled 0 lholed [Trap] es\<rbrakk> \<Longrightarrow> \<lparr>es\<rparr> \<leadsto> \<lparr>[Trap]\<rparr>"
@@ -185,7 +185,7 @@ inductive reduce :: "[s, f, e list, s, f, e list] \<Rightarrow> bool" ("\<lparr>
 | call_indirect_Some:"\<lbrakk>(f_inst f) = i; stab s i (nat_of_int c) = Some cl; stypes s i j = tf; cl_type cl = tf\<rbrakk> \<Longrightarrow> \<lparr>s;f;[$C (ConstInt32 c), $(Call_indirect j)]\<rparr> \<leadsto> \<lparr>s;f;[Invoke cl]\<rparr>"
 | call_indirect_None:"\<lbrakk>(f_inst f) = i; (stab s i (nat_of_int c) = Some cl \<and> stypes s i j \<noteq> cl_type cl) \<or> stab s i (nat_of_int c) = None\<rbrakk> \<Longrightarrow> \<lparr>s;f;[$C (ConstInt32 c), $(Call_indirect j)]\<rparr> \<leadsto> \<lparr>s;f;[Trap]\<rparr>"
   \<comment> \<open>\<open>invoke\<close>\<close>
-| invoke_native:"\<lbrakk>cl = Func_native j (t1s _> t2s) ts es; ves = ($C* vcs); length vcs = n; length ts = k; length t1s = n; length t2s = m; (n_zeros ts = zs) \<rbrakk> \<Longrightarrow> \<lparr>s;f;ves @ [Invoke cl]\<rparr> \<leadsto> \<lparr>s;f;[Local m \<lparr> f_locs = vcs@zs, f_inst = j \<rparr> [$(Block ([] _> t2s) es)]]\<rparr>"
+| invoke_native:"\<lbrakk>cl = Func_native j (t1s _> t2s) ts es; ves = ($C* vcs); length vcs = n; length ts = k; length t1s = n; length t2s = m; (n_zeros ts = zs) \<rbrakk> \<Longrightarrow> \<lparr>s;f;ves @ [Invoke cl]\<rparr> \<leadsto> \<lparr>s;f;[Frame m \<lparr> f_locs = vcs@zs, f_inst = j \<rparr> [$(Block ([] _> t2s) es)]]\<rparr>"
 | invoke_host_Some:"\<lbrakk>cl = Func_host (t1s _> t2s) h; ves = ($C* vcs); length vcs = n; length t1s = n; length t2s = m; host_apply s (t1s _> t2s) h vcs hs = Some (s', vcs')\<rbrakk> \<Longrightarrow> \<lparr>s;f;ves @ [Invoke cl]\<rparr> \<leadsto> \<lparr>s';f;($C* vcs')\<rparr>"
 | invoke_host_None:"\<lbrakk>cl = Func_host (t1s _> t2s) h; ves = ($C* vcs); length vcs = n; length t1s = n; length t2s = m\<rbrakk> \<Longrightarrow> \<lparr>s;f;ves @ [Invoke cl]\<rparr> \<leadsto> \<lparr>s;f;[Trap]\<rparr>"
   \<comment> \<open>\<open>get_local\<close>\<close>
@@ -218,7 +218,7 @@ inductive reduce :: "[s, f, e list, s, f, e list] \<Rightarrow> bool" ("\<lparr>
   \<comment> \<open>\<open>inductive label reduction\<close>\<close>
 | label:"\<lbrakk>\<lparr>s;f;es\<rparr> \<leadsto> \<lparr>s';f';es'\<rparr>; Lfilled k lholed es les; Lfilled k lholed es' les'\<rbrakk> \<Longrightarrow> \<lparr>s;f;les\<rparr> \<leadsto> \<lparr>s';f';les'\<rparr>"
   \<comment> \<open>\<open>inductive local reduction\<close>\<close>
-| local:"\<lbrakk>\<lparr>s;f;es\<rparr> \<leadsto> \<lparr>s';f';es'\<rparr>\<rbrakk> \<Longrightarrow> \<lparr>s;f0;[Local n f es]\<rparr> \<leadsto> \<lparr>s';f0;[Local n f' es']\<rparr>"
+| local:"\<lbrakk>\<lparr>s;f;es\<rparr> \<leadsto> \<lparr>s';f';es'\<rparr>\<rbrakk> \<Longrightarrow> \<lparr>s;f0;[Frame n f es]\<rparr> \<leadsto> \<lparr>s';f0;[Frame n f' es']\<rparr>"
 
 definition reduce_trans where
   "reduce_trans \<equiv> (\<lambda>(s,f,es) (s',f',es'). \<lparr>s;f;es\<rparr> \<leadsto> \<lparr>s';f';es'\<rparr>)^**"
